started translation of instructions to bitflags, other minor changes

Jolt/ConstraintSystem/Trace.lean
@@ -96,4 +96,319 @@ structure Device where
   memoryLayout : MemoryLayout
 deriving Repr, Inhabited, DecidableEq
 
+
+section Enum
+
+/- Defining `enum`s relevant for trace generation and R1CS -/
+
+section Memory
+
+inductive MemoryOpRead where
+  | RS1_Read
+  | RS2_Read
+  | RD_Read
+  | RAM_Read_Byte0
+  | RAM_Read_Byte1
+  | RAM_Read_Byte2
+  | RAM_Read_Byte3
+deriving Repr, Inhabited, DecidableEq
+
+def MemoryOpRead.toFin (mOp : MemoryOpRead) : Fin MEMORY_OPS_PER_INSTRUCTION :=
+  match mOp with
+  | RS1_Read => 0
+  | RS2_Read => 1
+  | RD_Read => 2
+  | RAM_Read_Byte0 => 3
+  | RAM_Read_Byte1 => 4
+  | RAM_Read_Byte2 => 5
+  | RAM_Read_Byte3 => 6
+
+instance : Coe MemoryOpRead (Fin MEMORY_OPS_PER_INSTRUCTION) := ⟨MemoryOpRead.toFin⟩
+
+instance : Equiv MemoryOpRead (Fin MEMORY_OPS_PER_INSTRUCTION) where
+  toFun := MemoryOpRead.toFin
+  invFun := fun n => MemoryOpRead.ofNat (n : Nat)
+  left_inv := by intro x ; rcases x <;> decide
+  right_inv := by decide
+
+-- instance : FinEnum MemoryOpRead := ⟨MEMORY_OPS_PER_INSTRUCTION, instEquivMemoryOpReadFinOfNatNat⟩
+
+instance : Fintype MemoryOpRead :=
+  Fintype.ofEquiv (Fin MEMORY_OPS_PER_INSTRUCTION) instEquivMemoryOpReadFinOfNatNat.symm
+
+@[simp]
+lemma MemoryOpRead_card : Fintype.card MemoryOpRead = MEMORY_OPS_PER_INSTRUCTION :=
+  by simp [Fintype.ofEquiv_card]
+
+
+inductive MemoryOpWrite where
+  | RD_Write
+  | RAM_Write_Byte0
+  | RAM_Write_Byte1
+  | RAM_Write_Byte2
+  | RAM_Write_Byte3
+deriving Repr, Inhabited, DecidableEq
+
+def MemoryOpWrite.toFin (mOp : MemoryOpWrite) : Fin NUM_MEM_WRITES :=
+  match mOp with
+  | RD_Write => 0
+  | RAM_Write_Byte0 => 1
+  | RAM_Write_Byte1 => 2
+  | RAM_Write_Byte2 => 3
+  | RAM_Write_Byte3 => 4
+
+instance : Coe MemoryOpWrite (Fin NUM_MEM_WRITES) := ⟨MemoryOpWrite.toFin⟩
+
+instance : Equiv MemoryOpWrite (Fin NUM_MEM_WRITES) where
+  toFun := MemoryOpWrite.toFin
+  invFun := fun n => MemoryOpWrite.ofNat (n : Nat)
+  left_inv := by intro x ; rcases x <;> decide
+  right_inv := by decide
+
+instance : Fintype MemoryOpWrite :=
+  Fintype.ofEquiv (Fin NUM_MEM_WRITES) instEquivMemoryOpWriteFinOfNatNat.symm
+
+@[simp]
+lemma MemoryOpWrite_card : Fintype.card MemoryOpWrite = NUM_MEM_WRITES := by
+  simp [Fintype.ofEquiv_card]
+
+end Memory
+
+section Bytecode
+
+inductive BytecodeValues where
+  | ELFAddress
+  | Bitflags
+  | RS1
+  | RS2
+  | RD
+  | Imm
+deriving Repr, Inhabited, DecidableEq
+
+def BytecodeValues.toFin (bValue : BytecodeValues) : Fin NUM_BYTECODE_VALUE_FIELDS :=
+  match bValue with
+  | BytecodeValues.ELFAddress => 0
+  | BytecodeValues.Bitflags => 1
+  | BytecodeValues.RS1 => 2
+  | BytecodeValues.RS2 => 3
+  | BytecodeValues.RD => 4
+  | BytecodeValues.Imm => 5
+
+instance : Coe BytecodeValues (Fin NUM_BYTECODE_VALUE_FIELDS) := ⟨BytecodeValues.toFin⟩
+
+instance : Equiv BytecodeValues (Fin NUM_BYTECODE_VALUE_FIELDS) where
+  toFun := BytecodeValues.toFin
+  invFun := fun n => BytecodeValues.ofNat (n : Nat)
+  left_inv := by intro x ; rcases x <;> decide
+  right_inv := by decide
+
+instance : Fintype BytecodeValues :=
+  Fintype.ofEquiv (Fin NUM_BYTECODE_VALUE_FIELDS) instEquivBytecodeValuesFinOfNatNat.symm
+
+@[simp]
+lemma BytecodeValues_card : Fintype.card BytecodeValues = NUM_BYTECODE_VALUE_FIELDS := by
+  simp [Fintype.ofEquiv_card]
+
+end Bytecode
+
+section Flags
+
+inductive CircuitFlags where
+  | OpFlags_IsRs1Rs2
+  | OpFlags_IsImm
+  | OpFlags_IsLoad
+  | OpFlags_IsStore
+  | OpFlags_IsJmp
+  | OpFlags_IsBranch
+  | OpFlags_LookupOutToRd
+  | OpFlags_SignImm
+  | OpFlags_IsConcat
+  | OpFlags_IsVirtualSequence
+  | OpFlags_IsVirtual
+deriving Repr, Inhabited, DecidableEq
+
+def CircuitFlags.toFin (cFlag : CircuitFlags) : Fin NUM_CIRCUIT_FLAGS :=
+  match cFlag with
+  | OpFlags_IsRs1Rs2 => 0
+  | OpFlags_IsImm => 1
+  | OpFlags_IsLoad => 2
+  | OpFlags_IsStore => 3
+  | OpFlags_IsJmp => 4
+  | OpFlags_IsBranch => 5
+  | OpFlags_LookupOutToRd => 6
+  | OpFlags_SignImm => 7
+  | OpFlags_IsConcat => 8
+  | OpFlags_IsVirtualSequence => 9
+  | OpFlags_IsVirtual => 10
+
+instance : Coe CircuitFlags (Fin NUM_CIRCUIT_FLAGS) := ⟨CircuitFlags.toFin⟩
+
+instance : Equiv CircuitFlags (Fin NUM_CIRCUIT_FLAGS) where
+  toFun := CircuitFlags.toFin
+  invFun := fun n => CircuitFlags.ofNat (n : Nat)
+  left_inv := by intro x ; rcases x <;> decide
+  right_inv := by decide
+
+instance : Fintype CircuitFlags :=
+  Fintype.ofEquiv (Fin NUM_CIRCUIT_FLAGS) instEquivCircuitFlagsFinOfNatNat.symm
+
+@[simp]
+lemma CircuitFlags_card : Fintype.card CircuitFlags = NUM_CIRCUIT_FLAGS := by
+  simp [Fintype.ofEquiv_card]
+
+inductive InstructionFlags where
+  | IF_Add
+  | IF_Sub
+  | IF_And
+  | IF_Or
+  | IF_Xor
+  | IF_Lb
+  | IF_Lh
+  | IF_Sb
+  | IF_Sh
+  | IF_Sw
+  | IF_Beq
+  | IF_Bge
+  | IF_Bgeu
+  | IF_Bne
+  | IF_Slt
+  | IF_Sltu
+  | IF_Sll
+  | IF_Sra
+  | IF_Srl
+  | IF_Movsign
+  | IF_Mul
+  | IF_MulU
+  | IF_MulHu
+  | IF_Virt_Adv
+  | IF_Virt_Assert_LTE
+  | IF_Virt_Assert_VALID_SIGNED_REMAINDER
+  | IF_Virt_Assert_VALID_UNSIGNED_REMAINDER
+  | IF_Virt_Assert_VALID_DIV0
+deriving Repr, Inhabited, DecidableEq
+
+def InstructionFlags.toFin (iFlag : InstructionFlags) : Fin NUM_INSTRUCTION_FLAGS :=
+  match iFlag with
+  | IF_Add => 0
+  | IF_Sub => 1
+  | IF_And => 2
+  | IF_Or => 3
+  | IF_Xor => 4
+  | IF_Lb => 5
+  | IF_Lh => 6
+  | IF_Sb => 7
+  | IF_Sh => 8
+  | IF_Sw => 9
+  | IF_Beq => 10
+  | IF_Bge => 11
+  | IF_Bgeu => 12
+  | IF_Bne => 13
+  | IF_Slt => 14
+  | IF_Sltu => 15
+  | IF_Sll => 16
+  | IF_Sra => 17
+  | IF_Srl => 18
+  | IF_Movsign => 19
+  | IF_Mul => 20
+  | IF_MulU => 21
+  | IF_MulHu => 22
+  | IF_Virt_Adv => 23
+  | IF_Virt_Assert_LTE => 24
+  | IF_Virt_Assert_VALID_SIGNED_REMAINDER => 25
+  | IF_Virt_Assert_VALID_UNSIGNED_REMAINDER => 26
+  | IF_Virt_Assert_VALID_DIV0 => 27
+
+instance : Coe InstructionFlags (Fin NUM_INSTRUCTION_FLAGS) := ⟨InstructionFlags.toFin⟩
+
+instance : Equiv InstructionFlags (Fin NUM_INSTRUCTION_FLAGS) where
+  toFun := InstructionFlags.toFin
+  invFun := fun n => InstructionFlags.ofNat (n : Nat)
+  left_inv := by intro x ; rcases x <;> decide
+  right_inv := by decide
+
+instance : Fintype InstructionFlags :=
+  Fintype.ofEquiv (Fin NUM_INSTRUCTION_FLAGS) instEquivInstructionFlagsFinOfNatNat.symm
+
+@[simp]
+lemma InstructionFlags_card : Fintype.card InstructionFlags = NUM_INSTRUCTION_FLAGS := by
+  simp [Fintype.ofEquiv_card]
+
+end Flags
+
+end Enum
+
+section Generation
+
+/- Generate traces from ELF instructions -/
+
+/-- Generate the circuit flags for a given `opcode`. TODO: figure out exact mapping -/
+def CircuitFlags.fromOpcode (opcode : RV32IM.Instr) : List CircuitFlags :=
+  match opcode with
+  | RV32IM.Instr.I (RV32I.Instr.ADD) => [OpFlags_IsRs1Rs2, OpFlags_IsImm]
+  | RV32IM.Instr.I (RV32I.Instr.SUB) => [OpFlags_IsRs1Rs2, OpFlags_IsImm]
+  | RV32IM.Instr.I (RV32I.Instr.AND) => [OpFlags_IsRs1Rs2, OpFlags_IsImm]
+  | RV32IM.Instr.I (RV32I.Instr.OR) => [OpFlags_IsRs1Rs2, OpFlags_IsImm]
+  | RV32IM.Instr.I (RV32I.Instr.XOR) => [OpFlags_IsRs1Rs2, OpFlags_IsImm]
+  -- For now, all other instructions are virtual
+  | _ => [OpFlags_IsVirtual]
+
+/-- Generate the instruction flag for a given `opcode`. TODO: figure out exact mapping -/
+def InstructionFlags.fromOpcode (opcode : RV32IM.Instr) : InstructionFlags :=
+  match opcode with
+  | RV32IM.Instr.I (RV32I.Instr.ADD) => IF_Add
+  | RV32IM.Instr.I (RV32I.Instr.SUB) => IF_Sub
+  | RV32IM.Instr.I (RV32I.Instr.AND) => IF_And
+  | RV32IM.Instr.I (RV32I.Instr.OR) => IF_Or
+  | RV32IM.Instr.I (RV32I.Instr.XOR) => IF_Xor
+  | RV32IM.Instr.I (RV32I.Instr.LB) => IF_Lb
+  | RV32IM.Instr.I (RV32I.Instr.LH) => IF_Lh
+  | RV32IM.Instr.I (RV32I.Instr.SB) => IF_Sb
+  | RV32IM.Instr.I (RV32I.Instr.SH) => IF_Sh
+  | RV32IM.Instr.I (RV32I.Instr.SW) => IF_Sw
+  | RV32IM.Instr.I (RV32I.Instr.BEQ) => IF_Beq
+  | RV32IM.Instr.I (RV32I.Instr.BGE) => IF_Bge
+  | RV32IM.Instr.I (RV32I.Instr.BGEU) => IF_Bgeu
+  | RV32IM.Instr.I (RV32I.Instr.BNE) => IF_Bne
+  | RV32IM.Instr.I (RV32I.Instr.SLT) => IF_Slt
+  | RV32IM.Instr.I (RV32I.Instr.SLTU) => IF_Sltu
+  | RV32IM.Instr.I (RV32I.Instr.SLL) => IF_Sll
+  | RV32IM.Instr.I (RV32I.Instr.SRA) => IF_Sra
+  | RV32IM.Instr.I (RV32I.Instr.SRL) => IF_Srl
+  | RV32IM.Instr.I (RV32I.Instr.SRAI) => IF_Sra
+  | RV32IM.Instr.I (RV32I.Instr.SRLI) => IF_Srl
+  -- Not sure if these two are correct
+  | RV32IM.Instr.I (RV32I.Instr.JAL) => IF_Movsign
+  | RV32IM.Instr.I (RV32I.Instr.JALR) => IF_Movsign
+  -- the rest just goes to this one for now
+  | _ => IF_Virt_Adv
+  -- | IF_Mul => 20
+  -- | IF_MulU => 21
+  -- | IF_MulHu => 22
+  -- | IF_Virt_Adv => 23
+  -- | IF_Virt_Assert_LTE => 24
+  -- | IF_Virt_Assert_VALID_SIGNED_REMAINDER => 25
+  -- | IF_Virt_Assert_VALID_UNSIGNED_REMAINDER => 26
+  -- | IF_Virt_Assert_VALID_DIV0 => 27
+
+
+/-- Pack the circuit flags and instruction flags into a single bitflag. The circuit flags are the higher bits, and the instruction flags are the lower bits.
+TODO: prove that the modulo `UInt64` does not overflow -/
+def packBitflags (cFlags : List CircuitFlags) (iFlag : InstructionFlags) : UInt64 :=
+  let packedFlags := cFlags.foldl (fun acc flag => acc + (1 <<< flag.toFin)) (1 <<< iFlag.toFin)
+  packedFlags.toUInt64
+
+
+/-- Generate `Bytecode.Row` from `ELFInstruction`. For now, we ignore the `virtualSequenceIndex` field which is only relevant for a few instructions. -/
+def Bytecode.Row.fromELFInstruction (instr : ELFInstruction) : Bytecode.Row where
+  address := instr.address.toUSize
+  bitflags := packBitflags (CircuitFlags.fromOpcode instr.opcode) (InstructionFlags.fromOpcode instr.opcode)
+  rs1 := instr.rs1.getD 0
+  rs2 := instr.rs2.getD 0
+  rd := instr.rd.getD 0
+  imm := (instr.imm.getD 0).toUInt64
+
+
+end Generation
+
+
 end Jolt
